src/cbor/CBOR.SteelST.Raw.Array.fsti
@@ -1,0 +1,128 @@
+module CBOR.SteelST.Raw.Array
+include CBOR.SteelST.Raw.Base
+open CBOR.SteelST.Raw.Validate
+open LowParse.SteelST.Combinators
+open LowParse.SteelST.Recursive
+open LowParse.SteelST.BitSum
+open LowParse.SteelST.ValidateAndRead
+open Steel.ST.GenElim
+
+module AP = LowParse.SteelST.ArrayPtr
+module SZ = FStar.SizeT
+module R = Steel.ST.Reference
+module NL = LowParse.SteelST.VCList.Sorted
+module U8 = FStar.UInt8
+module U64 = FStar.UInt64
+
+unfold
+let get_raw_data_item_payload_array_post
+  (va: v parse_raw_data_item_kind raw_data_item)
+  (vh: v (get_parser_kind parse_header) header)
+  (n: nat)
+  (vc: v (NL.parse_nlist_kind n parse_raw_data_item_kind) (NL.nlist n raw_data_item))
+: GTot prop
+=
+        let (| h, c |) = synth_raw_data_item_recip va.contents in
+        let (| b, x |) = h in
+        // order of the following conjuncts matters for typechecking
+        vh.contents == h /\
+        n == UInt64.v (argument_as_uint64 b x) /\
+        va.contents == Array vc.contents /\
+        vc.contents == c /\
+        AP.merge_into (array_of' vh) (array_of' vc) (array_of va)
+
+val get_raw_data_item_payload_array
+  (#opened: _)
+  (#va: v parse_raw_data_item_kind raw_data_item)
+  (a: byte_array)
+: STGhost (Ghost.erased byte_array) opened
+    (aparse parse_raw_data_item a va)
+    (fun a' -> exists_ (fun vh -> exists_ (fun (n: nat) -> exists_ (fun vc ->
+      aparse parse_header a vh `star`
+      aparse (NL.parse_nlist n parse_raw_data_item) a' vc `star`
+      pure (get_raw_data_item_payload_array_post va vh n vc)
+    ))))
+    (Array? va.contents)
+    (fun _ -> True)
+
+val intro_raw_data_item_array
+  (#opened: _)
+  (#vh: v (get_parser_kind parse_header) header)
+  (h: byte_array)
+  (#n: nat)
+  (#vc: v (NL.parse_nlist_kind n parse_raw_data_item_kind) (NL.nlist n raw_data_item))
+  (c: byte_array)
+: STGhost (v parse_raw_data_item_kind raw_data_item) opened
+    (aparse parse_header h vh `star`
+      aparse (NL.parse_nlist n parse_raw_data_item) c vc
+    )
+    (fun va -> aparse parse_raw_data_item h va)
+    (
+      let (| b, x |) = vh.contents in
+      let (major_type, _) = b in
+      n == UInt64.v (argument_as_uint64 b x) /\
+      major_type == get_major_type (Array vc.contents) /\
+      AP.adjacent (array_of' vh) (array_of' vc)
+    )
+    (fun va ->
+      get_raw_data_item_payload_array_post va vh n vc
+    )
+
+let focus_array_with_ghost_length_post
+  (n: nat)
+  (va: v parse_raw_data_item_kind raw_data_item)
+  (vres: v (NL.parse_nlist_kind n parse_raw_data_item_kind) (NL.nlist n raw_data_item))
+: Tot prop
+= Array? va.contents /\
+  Array?.v va.contents == vres.contents
+
+val focus_array_with_ghost_length
+  (n: Ghost.erased nat)
+  (#va: v parse_raw_data_item_kind raw_data_item)
+  (a: byte_array)
+: ST byte_array
+    (aparse parse_raw_data_item a va)
+    (fun res -> exists_ (fun vres ->
+      aparse (NL.parse_nlist n parse_raw_data_item) res vres `star`
+      (aparse (NL.parse_nlist n parse_raw_data_item) res vres `implies_`
+        aparse parse_raw_data_item a va
+      ) `star` pure (
+      focus_array_with_ghost_length_post n va vres
+    )))
+    (Array? va.contents /\
+      Ghost.reveal n == List.Tot.length (Array?.v va.contents)
+    )
+    (fun _ -> True)
+
+[@@erasable]
+noeq
+type focus_array_res = {
+  n: U64.t;
+  l: v (NL.parse_nlist_kind (U64.v n) parse_raw_data_item_kind) (NL.nlist (U64.v n) raw_data_item);
+  a: byte_array;
+}
+
+val focus_array
+  (#n': Ghost.erased U64.t)
+  (#a': Ghost.erased byte_array)
+  (#va: v parse_raw_data_item_kind raw_data_item)
+  (pn: R.ref U64.t)
+  (pa: R.ref byte_array)
+  (a: byte_array)
+: ST focus_array_res
+    (aparse parse_raw_data_item a va `star`
+      R.pts_to pn full_perm n' `star`
+      R.pts_to pa full_perm a'
+    )
+    (fun res ->
+      R.pts_to pn full_perm res.n `star`
+      R.pts_to pa full_perm res.a `star`
+      aparse (NL.parse_nlist (U64.v res.n) parse_raw_data_item) res.a res.l `star`
+      (aparse (NL.parse_nlist (U64.v res.n) parse_raw_data_item) res.a res.l `implies_`
+        aparse parse_raw_data_item a va
+      )
+    )
+    (Array? va.contents)
+    (fun res ->
+      va.contents == Array res.l.contents
+    )
