src/cbor/CBOR.SteelST.Raw.Map.fsti
@@ -1,0 +1,189 @@
+module CBOR.SteelST.Raw.Map
+include CBOR.SteelST.Raw.Base
+open CBOR.SteelST.Raw.Validate
+open LowParse.SteelST.Combinators
+open LowParse.SteelST.Assoc
+open LowParse.SteelST.Recursive
+open LowParse.SteelST.BitSum
+open LowParse.SteelST.ValidateAndRead
+open LowParse.SteelST.SeqBytes
+open Steel.ST.GenElim
+
+module AP = LowParse.SteelST.ArrayPtr
+module SZ = FStar.SizeT
+module R = Steel.ST.Reference
+module NL = LowParse.SteelST.VCList.Sorted
+module SB = LowParse.SteelST.SeqBytes
+module U8 = FStar.UInt8
+module Cast = FStar.Int.Cast
+module I16 = FStar.Int16
+module U16 = FStar.UInt16
+module U32 = FStar.UInt32
+module U64 = FStar.UInt64
+
+#set-options "--ide_id_info_off"
+
+(* 4.2 Ordering of map keys *)
+
+inline_for_extraction
+noextract
+val map_entry_order_impl
+  (#kkey: Ghost.erased parser_kind)
+  (#key: Type0)
+  (pkey: parser kkey key)
+  (#key_order: Ghost.erased (key -> key -> bool))
+  (key_order_impl: NL.order_impl pkey key_order)
+  (#kvalue: Ghost.erased parser_kind)
+  (#value: Type0)
+  (pvalue: parser kvalue value)
+: Pure (NL.order_impl (pkey `nondep_then` pvalue) (map_entry_order key_order value))
+    (requires (kkey.parser_kind_subkind == Some ParserStrong))
+    (ensures (fun _ -> True))
+
+unfold
+let get_raw_data_item_payload_map_post
+  (va: v parse_raw_data_item_kind raw_data_item)
+  (vh: v (get_parser_kind parse_header) header)
+  (n: nat)
+  (vc: v (NL.parse_nlist_kind n (and_then_kind parse_raw_data_item_kind parse_raw_data_item_kind)) (NL.nlist n (raw_data_item & raw_data_item)))
+: GTot prop
+=
+        let (| h, c |) = synth_raw_data_item_recip va.contents in
+        let (| b, x |) = h in
+        // order of the following conjuncts matters for typechecking
+        vh.contents == h /\
+        n == UInt64.v (argument_as_uint64 b x) /\
+        va.contents == Map vc.contents /\
+        vc.contents == c /\
+        AP.merge_into (array_of' vh) (array_of' vc) (array_of va)
+
+val get_raw_data_item_payload_map
+  (#opened: _)
+  (#va: v parse_raw_data_item_kind raw_data_item)
+  (a: byte_array)
+: STGhost (Ghost.erased byte_array) opened
+    (aparse parse_raw_data_item a va)
+    (fun a' -> exists_ (fun vh -> exists_ (fun (n: nat) -> exists_ (fun vc ->
+      aparse parse_header a vh `star`
+      aparse (NL.parse_nlist n (parse_raw_data_item `nondep_then` parse_raw_data_item)) a' vc `star`
+      pure (get_raw_data_item_payload_map_post va vh n vc)
+    ))))
+    (Map? va.contents)
+    (fun _ -> True)
+
+val intro_raw_data_item_map
+  (#opened: _)
+  (#vh: v (get_parser_kind parse_header) header)
+  (h: byte_array)
+  (#n: nat)
+  (#vc: v (NL.parse_nlist_kind n (and_then_kind parse_raw_data_item_kind parse_raw_data_item_kind)) (NL.nlist n (raw_data_item & raw_data_item)))
+  (c: byte_array)
+: STGhost (v parse_raw_data_item_kind raw_data_item) opened
+    (aparse parse_header h vh `star`
+      aparse (NL.parse_nlist n (parse_raw_data_item `nondep_then` parse_raw_data_item)) c vc
+    )
+    (fun va -> aparse parse_raw_data_item h va)
+    (
+      let (| b, x |) = vh.contents in
+      let (major_type, _) = b in
+      n == UInt64.v (argument_as_uint64 b x) /\
+      major_type == get_major_type (Map vc.contents) /\
+      AP.adjacent (array_of' vh) (array_of' vc)
+    )
+    (fun va ->
+      get_raw_data_item_payload_map_post va vh n vc
+    )
+
+noextract
+let focus_map_postcond
+  (va: v parse_raw_data_item_kind raw_data_item)
+  (n: nat)
+  (va': v (NL.parse_nlist_kind n (and_then_kind parse_raw_data_item_kind parse_raw_data_item_kind)) (NL.nlist n (raw_data_item & raw_data_item)))
+: Tot prop
+= Map? va.contents /\
+  va'.contents == Map?.v va.contents
+
+val focus_map_with_ghost_length
+  (#va: v parse_raw_data_item_kind raw_data_item)
+  (a: byte_array)
+  (n: Ghost.erased nat)
+: ST byte_array
+    (aparse parse_raw_data_item a va)
+    (fun a' -> exists_ (fun va' ->
+      aparse (NL.parse_nlist n (parse_raw_data_item `nondep_then` parse_raw_data_item)) a' va' `star`
+
+      (aparse (NL.parse_nlist n (parse_raw_data_item `nondep_then` parse_raw_data_item)) a' va' `implies_`
+        aparse parse_raw_data_item a va) `star`
+      pure (focus_map_postcond va n va')
+    ))
+    (Map? va.contents /\
+      Ghost.reveal n == List.Tot.length (Map?.v va.contents)
+    )
+    (fun _ -> True)
+
+inline_for_extraction
+noextract
+val check_data_item_wf_head
+  (#order: Ghost.erased (raw_data_item -> raw_data_item -> bool))
+  (order_impl: NL.order_impl parse_raw_data_item order)
+  (sq: squash (SZ.fits_u64))
+: Tot (pred_recursive_base_t serialize_raw_data_item_param (data_item_wf_head order))
+
+inline_for_extraction
+noextract
+val check_raw_data_item
+  (#p: Ghost.erased (raw_data_item -> bool))
+  (p_impl: pred_recursive_base_t serialize_raw_data_item_param p)
+  (#va: v parse_raw_data_item_kind raw_data_item)
+  (a: byte_array)
+: ST bool
+    (aparse parse_raw_data_item a va)
+    (fun _ -> aparse parse_raw_data_item a va)
+    True
+    (fun res -> res == holds_on_raw_data_item p va.contents)
+
+inline_for_extraction
+noextract
+val validate_raw_data_item_filter
+  (#p: Ghost.erased (raw_data_item -> bool))
+  (p_impl: pred_recursive_base_t serialize_raw_data_item_param p)
+: Tot (validator (parse_filter parse_raw_data_item (holds_on_raw_data_item p)))
+
+inline_for_extraction
+noextract
+val validate_data_item
+  (#order: Ghost.erased (raw_data_item -> raw_data_item -> bool))
+  (order_impl: NL.order_impl parse_raw_data_item order)
+: Tot (validator (parse_data_item order))
+
+val deterministically_encoded_cbor_map_key_order_impl
+: NL.order_impl parse_raw_data_item deterministically_encoded_cbor_map_key_order
+
+val validate_deterministically_encoded_cbor_data_item
+: validator (parse_data_item deterministically_encoded_cbor_map_key_order)
+
+inline_for_extraction // necessary for the reexport into CBOR.SteelST
+val validate_canonical_cbor_data_item
+: validator (parse_data_item canonical_cbor_map_key_order)
+
+val jump_data_item
+  (order: Ghost.erased (raw_data_item -> raw_data_item -> bool))
+: Tot (jumper (parse_data_item order))
+
+(* Comparisons with unserialized values *)
+
+val lex_compare_with_header
+  (ty: Ghost.erased major_type_t { ty `U8.lt` major_type_simple_value })
+  (x: U64.t)
+  (b: U8.t)
+  (#vh: v (get_parser_kind parse_header) header)
+  (a: byte_array)
+: ST I16.t
+    (aparse parse_header a vh)
+    (fun _ -> aparse parse_header a vh)
+    (b == get_uint64_as_initial_byte ty x)
+    (fun i ->
+      let s0 = serialize serialize_header (uint64_as_argument ty x) in
+      let s = serialize serialize_header vh.contents in
+      bytes_lex_compare s0 s `same_sign` I16.v i
+    )
