src/cbor/CBOR.SteelST.Raw.Write.fsti
@@ -1,0 +1,267 @@
+module CBOR.SteelST.Raw.Write
+include CBOR.SteelST.Raw.Base
+open CBOR.SteelST.Raw.Read
+open LowParse.SteelST.Combinators
+open LowParse.SteelST.Assoc
+open LowParse.SteelST.Recursive
+open LowParse.SteelST.BitSum
+open LowParse.SteelST.ValidateAndRead
+open LowParse.SteelST.SeqBytes
+open Steel.ST.GenElim
+
+module R = Steel.ST.Reference
+module AP = LowParse.SteelST.ArrayPtr
+module SZ = FStar.SizeT
+module R = Steel.ST.Reference
+module NL = LowParse.SteelST.VCList.Sorted
+module SB = LowParse.SteelST.SeqBytes
+module U8 = FStar.UInt8
+module Cast = FStar.Int.Cast
+module I16 = FStar.Int16
+module U64 = FStar.UInt64
+
+#set-options "--ide_id_info_off"
+
+(* Writers *)
+
+val write_initial_byte
+  (t: major_type_t)
+  (x: additional_info_t)
+  (sq: squash (
+    initial_byte_wf (t, (x, ()))
+  ))
+  (#va: AP.v byte)
+  (a: byte_array)
+: ST (v (get_parser_kind parse_initial_byte) initial_byte)
+    (AP.arrayptr a va)
+    (fun va' ->
+      aparse parse_initial_byte a va'
+    )
+    (AP.length (AP.array_of va) == 1 /\
+      AP.array_perm (AP.array_of va) == full_perm
+    )
+    (fun va' -> 
+       array_of' va' == AP.array_of va /\
+       va'.contents == mk_initial_byte t x
+    )
+
+inline_for_extraction
+noextract
+val write_initial_byte'
+: exact_writer serialize_initial_byte
+
+inline_for_extraction
+noextract
+val write_long_argument
+  (b: initial_byte)
+  (a: long_argument b)
+: Tot (maybe_r2l_writer_for (serialize_long_argument b) a)
+
+inline_for_extraction
+noextract
+val size_comp_long_argument
+  (b: initial_byte)
+  (a: long_argument b)
+: Tot (size_comp_for (serialize_long_argument b) a)
+
+inline_for_extraction
+noextract
+val l2r_write_long_argument
+  (b: initial_byte)
+  (a: long_argument b)
+: Tot (l2r_writer_for (serialize_long_argument b) a)
+
+inline_for_extraction
+noextract
+val write_header : maybe_r2l_writer serialize_header
+
+inline_for_extraction
+noextract
+val size_comp_header : size_comp serialize_header
+
+inline_for_extraction
+noextract
+val l2r_write_header : l2r_writer serialize_header
+
+inline_for_extraction
+noextract
+val write_simple_value_as_argument
+  (x: simple_value)
+: Tot (maybe_r2l_writer_for serialize_header (simple_value_as_argument x))
+
+inline_for_extraction
+noextract
+val size_comp_simple_value_as_argument
+  (x: simple_value)
+: Tot (size_comp_for serialize_header (simple_value_as_argument x))
+
+inline_for_extraction
+noextract
+val l2r_write_simple_value_as_argument
+  (x: simple_value)
+: Tot (l2r_writer_for serialize_header (simple_value_as_argument x))
+
+module W = LowParse.SteelST.R2LOutput
+
+val maybe_r2l_write_simple_value
+  (#opened: _)
+  (x: simple_value)
+  (#vout: _)
+  (out: W.t)
+  (success: bool)
+: STGhostT unit opened
+   (maybe_r2l_write serialize_header out vout (simple_value_as_argument x) success)
+   (fun _ -> maybe_r2l_write serialize_raw_data_item out vout (Simple x) success)
+
+inline_for_extraction // necessary for the reexport into CBOR.SteelST
+val write_simple_value
+  (x: simple_value)
+: Tot (maybe_r2l_writer_for serialize_raw_data_item (Simple x))
+
+val write_uint64_as_argument
+  (ty: major_type_t { ty `U8.lt` major_type_simple_value })
+  (x: U64.t)
+: Tot (maybe_r2l_writer_for serialize_header (uint64_as_argument ty x))
+
+inline_for_extraction
+noextract
+val size_comp_simple_value_header
+  (x: simple_value)
+: Tot (size_comp_for serialize_header (simple_value_as_argument x))
+
+val size_comp_simple_value
+  (x: simple_value)
+: Tot (size_comp_for serialize_raw_data_item (Simple x))
+
+inline_for_extraction
+noextract
+val l2r_write_simple_value_header
+  (x: simple_value)
+: Tot (l2r_writer_for serialize_header (simple_value_as_argument x))
+
+val l2r_write_simple_value
+  (x: simple_value)
+: Tot (l2r_writer_for serialize_raw_data_item (Simple x))
+
+val size_comp_uint64_header
+  (ty: major_type_t { ty `U8.lt` major_type_simple_value })
+  (x: U64.t)
+: Tot (size_comp_for serialize_header (uint64_as_argument ty x))
+
+val size_comp_int64
+  (ty: major_type_uint64_or_neg_int64)
+  (x: U64.t)
+: Tot (size_comp_for serialize_raw_data_item (Int64 ty x))
+
+val size_comp_string
+  (ty: major_type_byte_string_or_text_string)
+  (x: U64.t)
+  (v: Ghost.erased (Seq.seq byte) { Seq.length v == U64.v x /\ SZ.fits_u64 })
+: Tot (size_comp_for serialize_raw_data_item (String ty (Ghost.reveal v)))
+
+val l2r_write_uint64_header
+  (ty: major_type_t { ty `U8.lt` major_type_simple_value })
+  (x: U64.t)
+: Tot (l2r_writer_for serialize_header (uint64_as_argument ty x))
+
+val l2r_write_int64
+  (ty: major_type_uint64_or_neg_int64)
+  (x: U64.t)
+: Tot (l2r_writer_for serialize_raw_data_item (Int64 ty x))
+
+val maybe_r2l_write_int64
+  (#opened: _)
+  (m: major_type_uint64_or_neg_int64)
+  (x: U64.t)
+  (#vout: _)
+  (out: W.t)
+  (success: bool)
+: STGhostT unit opened
+   (maybe_r2l_write serialize_header out vout (uint64_as_argument m x) success)
+   (fun _ -> maybe_r2l_write serialize_raw_data_item out vout (Int64 m x) success)
+
+inline_for_extraction // necessary for the reexport into CBOR.SteelST
+val write_int64
+  (m: major_type_uint64_or_neg_int64)
+  (x: U64.t)
+: Tot (maybe_r2l_writer_for serialize_raw_data_item (Int64 m x))
+
+let finalize_raw_data_item_string_post_prop
+  (m: major_type_byte_string_or_text_string)
+  (va: v parse_raw_data_item_kind raw_data_item)
+  (vp: AP.v byte)
+: GTot prop
+=
+        FStar.UInt.fits (Seq.length (AP.contents_of vp)) U64.n /\
+        va.contents == String m (AP.contents_of vp)
+
+let finalize_raw_data_item_string_failure
+  (m: major_type_byte_string_or_text_string)
+  (vout: AP.array byte)
+  (vp: AP.v byte)
+: GTot prop
+= 
+  FStar.UInt.fits (Seq.length (AP.contents_of vp)) U64.n /\
+  Seq.length (serialize serialize_raw_data_item (String m (AP.contents_of vp))) > AP.length vout + AP.length (AP.array_of vp)
+
+[@@__reduce__]
+let finalize_raw_data_item_string_post
+  (m: major_type_byte_string_or_text_string)
+  (vout: AP.array byte)
+  (out: W.t)
+  (vp: AP.v byte)
+  (ap: byte_array)
+  (res: bool)
+: Tot vprop
+=
+      ifthenelse_vprop
+        res
+        (fun _ -> exists_ (fun vout' -> exists_ (fun a -> exists_ (fun va ->
+          aparse parse_raw_data_item a va `star`
+          W.vp out vout' `star`
+          pure (
+            AP.adjacent vout (AP.array_of vp) /\
+            AP.merge_into vout' (array_of va) (AP.merge vout (AP.array_of vp)) /\
+            finalize_raw_data_item_string_post_prop m va vp
+        )))))
+        (fun _ ->
+          pure (finalize_raw_data_item_string_failure m vout vp) `star`
+          W.vp out vout `star` AP.arrayptr ap vp
+        )
+
+val maybe_finalize_raw_data_item_string
+  (#opened: _)
+  (m: major_type_byte_string_or_text_string)
+  (#vout: _)
+  (out: W.t)
+  (#vp: _)
+  (ap: byte_array)
+  (len: U64.t)
+  (res: bool)
+: STGhost unit opened
+    (maybe_r2l_write serialize_header out vout (uint64_as_argument m len) res `star`
+      AP.arrayptr ap vp
+    )
+    (fun _ ->
+      finalize_raw_data_item_string_post m vout out vp ap res
+    )
+    (U64.v len == AP.length (AP.array_of vp) /\
+      AP.adjacent vout (AP.array_of vp)
+    )
+    (fun _ -> True)
+
+inline_for_extraction // necessary for the reexport into CBOR.SteelST
+val finalize_raw_data_item_string
+  (m: major_type_byte_string_or_text_string)
+  (#vout: _)
+  (out: W.t)
+  (#vp: _)
+  (ap: Ghost.erased byte_array)
+  (len: U64.t)
+: ST bool
+    (W.vp out vout `star` AP.arrayptr ap vp)
+    (fun res -> finalize_raw_data_item_string_post m vout out vp ap res)
+    (U64.v len == AP.length (AP.array_of vp) /\
+      AP.adjacent vout (AP.array_of vp)
+    )
+    (fun _ -> True)
